theories/Ext/ExprSubst.v
@@ -191,6 +191,100 @@ Section instantiate.
         autorewrite with exprD_rw.
         forward. } }
   Qed.
+
+  Lemma typeof_expr_instantiate_Some
+  : forall (*lookup : uvar -> option (expr func)*) (tu : list typ)
+           (tg : tenv typ),
+      (forall (u : uvar) (e' : expr func) t',
+         lookup u = Some e' ->
+         nth_error tu u = Some t' ->
+         typeof_expr tu tg e' = Some t') ->
+      forall (e : expr func) (tg' : list typ) t,
+        typeof_expr tu (tg' ++ tg) e = Some t ->
+        typeof_expr tu (tg' ++ tg) (instantiate (length tg') e) = Some t.
+  Proof.
+    clear. induction e; simpl; intros; auto; forward.
+    { eapply IHe1 in H0. eapply IHe2 in H1.
+      Cases.rewrite_all_goal. reflexivity. }
+    { inv_all; subst.
+      eapply (IHe (t :: tg')) in H0.
+      simpl in H0. rewrite H0. reflexivity. }
+    { eapply H in H1; eauto.
+      generalize (@typeof_expr_lift _ _ RSym_func tu nil tg' tg e).
+      simpl. congruence. }
+  Qed.
+
+  Lemma exprD'_instantiate_Some
+  : forall tus tvs P,
+      (forall u t' e get,
+         nth_error_get_hlist_nth _ tus u = Some (@existT _ _ t' get) ->
+         lookup u = Some e ->
+         exists eD,
+           exprD' tus tvs e t' = Some eD /\
+           forall us vs,
+             P us vs ->
+             eD us vs = get us) ->
+      forall e tvs' t eD,
+        exprD' tus (tvs' ++ tvs) e t = Some eD ->
+        exists eD',
+          exprD' tus (tvs' ++ tvs) (instantiate (length tvs') e) t = Some eD' /\
+          forall us vs' vs,
+            P us vs ->
+            eD us (hlist_app vs' vs) = eD' us (hlist_app vs' vs).
+  Proof.
+    clear.
+    induction e; simpl; intros; eauto.
+    { red_exprD.
+      forward; inv_all; subst.
+      specialize (IHe1 _ _ _ H2); clear H2.
+      specialize (IHe2 _ _ _ H3); clear H3.
+      eapply typeof_expr_instantiate_Some in H1; eauto.
+      { forward_reason.
+        Cases.rewrite_all_goal.
+        rewrite typ_cast_typ_refl. eexists; split; eauto.
+        simpl. intros.
+        rewrite H4; eauto.
+        rewrite H3; eauto. }
+      { clear - H.
+        intros.
+        specialize (H u t' e').
+        consider (nth_error_get_hlist_nth (typD ts nil) tus u); intros.
+        { destruct s.
+          generalize H.
+          eapply nth_error_get_hlist_nth_Some in H. simpl in *.
+          forward_reason.
+          rewrite x0 in H1. inv_all; subst.
+          intros.
+          specialize (H2 _ H1 H0). destruct H2 as [ ? [ ? ? ] ].
+          clear H H1.
+          rewrite exprD'_type_cast in H2.
+          forward. inv_all; subst. reflexivity. }
+        { exfalso. eapply nth_error_get_hlist_nth_None in H.
+          congruence. } } }
+    { red_exprD.
+      forward; inv_all; subst.
+      specialize (IHe (t :: tvs') t2 _ H2).
+      simpl in IHe.
+      forward_reason.
+      rewrite H0.
+      eexists; split; eauto.
+      simpl. intros.
+      eapply functional_extensionality. intros.
+      exact (H1 us (Hcons x0 vs') vs X). }
+    { consider (lookup u); intros.
+      { red_exprD.
+        forward; inv_all; subst.
+        specialize (H _ _ _ _ H2 H1).
+        forward_reason.
+        generalize (@exprD'_lift _ _ RSym_func tus nil tvs' tvs e t).
+        simpl. rewrite H.
+        intros. forward.
+        eexists; split; eauto.
+        intros.
+        erewrite <- H0. symmetry. eapply (H4 us Hnil vs' vs). apply X. }
+      { eauto. } }
+  Qed.
+
 End instantiate.
 
 Section mentionsU.
