theories/Util/Iteration.v
@@ -1,0 +1,48 @@
+Require Import Coq.Lists.List.
+Require Import ExtLib.Data.Option.
+Require Import ExtLib.Tactics.Consider.
+Require Import ExtLib.Tactics.Injection.
+
+Set Implicit Arguments.
+Set Strict Implicit.
+
+Section iteration.
+  Context (T U : Type) (f : T -> option U).
+
+  Fixpoint first_success  (ls : list T) : option U :=
+    match ls with
+      | nil => None
+      | l :: ls =>
+        match f l with
+          | None => first_success ls
+          | x => x
+        end
+    end.
+
+  Lemma first_success_sound
+  : forall ls val,
+      first_success ls = Some val ->
+      exists l,
+        In l ls /\ f l = Some val.
+  Proof.
+    induction ls; simpl; intros.
+    - congruence.
+    - consider (f a); intros.
+      + exists a. inv_all; subst. auto.
+      + apply IHls in H0. destruct H0. intuition. eauto.
+  Qed.
+
+  Variable (f' : T -> U -> option U).
+
+  Fixpoint all_success (ls : list T) (acc : U)
+  : option U :=
+    match ls with
+      | nil => Some acc
+      | l :: ls =>
+        match f' l acc with
+          | None => None
+          | Some x => all_success ls x
+        end
+    end.
+
+End iteration.
